pmap_skel.v
@@ -1,0 +1,767 @@
+Require Import GPUCSL.
+Require Import scan_lib.
+Require Import LibTactics.
+Require Import Skel_lemma.
+Require Import Psatz.
+
+Close Scope Qc_scope.
+Close Scope Q_scope.
+
+Section Map.
+(* variables *)
+Local Notation TID := (Var "tid").
+Local Notation BID := (Var "bid").
+Local Notation ARR := (Var "arr").
+Local Notation OUT := (Var "out").
+Local Notation X := (Var "x").
+Local Notation Y := (Var "y").
+Local Notation I := (Var "i").
+
+(* # of threads/blocks per block/grid *)
+Variable ntrd : nat.
+Variable nblk : nat.
+
+(* Variable arr : val. *)
+Variable len : nat.
+Hypothesis len_neq_0 : len <> 0.
+Variable out : list val.
+
+(* free variable environment (de-bruijn indices, dimensions) *)
+Variable env : list (nat * nat).
+
+(* dimensions of input and output arrays *)
+Variable inDim : nat.
+Variable outDim : nat.
+
+(* getter code of the input array *)
+Variable get : var -> (cmd * list exp).
+
+(* compiled code of the mapping function *)
+Variable func : list var -> (cmd * list exp).
+
+Hypothesis ntrd_neq0 : ntrd <> 0.
+Hypothesis nblk_neq0 : nblk <> 0.
+
+(* Variable f_ini : nat -> val. *)
+Variable fout : nat -> list val.
+
+(* local variables used by the template *)
+Definition xs := locals "x" inDim.
+
+(* auxilirary definition for written array *)
+Definition Outs := fst (fst (writeArray "Out" outDim Gl)).
+Definition Len := snd (fst (writeArray "Out" outDim Gl)).
+Definition setOut ix es := snd (writeArray "Out" outDim Gl) ix es.
+
+(* mapping templates *)
+Definition map_ker inv :=
+  I ::= (TID +C BID *C Z.of_nat ntrd);;
+  WhileI inv (I < Len) (
+    (fst (get I)) ;;
+    read_tup xs (snd (get I)) ;;
+    (fst (func xs)) ;;
+    catcmd (setOut I (snd (func xs))) ;;
+    I ::= I +C Z.of_nat ntrd *C Z.of_nat nblk
+  )%exp.
+
+Local Close Scope exp_scope.
+
+Local Notation nt_gr := (nblk * ntrd).
+
+Import ListNotations.
+
+(** runtime values *)
+(* runtime value of the input arrays: length * elements *)
+Variable env_den : list (list Z * nat * (nat -> list val)).
+
+(* env is consistent with env_den *)
+Hypothesis env_env_den_same_len : length env = length env_den.
+
+(* denotation of get *)
+Variable get_den : val -> list val.
+(* free variable conditions *)
+Hypothesis get_fv :
+  forall v, disjoint [I; BID] (writes_var (fst (get v))) .
+Hypothesis get_fv_sh :
+  forall u v, List.In u (writes_var (fst (get v))) -> prefix "sh" (var_of_str u) = false.
+Hypothesis get_fv_arr :
+  forall u v, List.In u (writes_var (fst (get v))) -> prefix "arr" (var_of_str u) = false.
+(* result expressions do not conflict with "x" prefixed variables *)
+Hypothesis get_res_fv :
+  forall v u e, In e (snd (get v)) -> In u (fv_E e) -> prefix "x" (var_of_str u) = false.
+(* get has no barriers *)
+Hypothesis get_no_bar :
+  forall v, barriers (fst (get v)) = nil.
+
+Hypothesis get_denote : forall (var : var) nt (tid : Fin.t nt) (val : val),
+  ~In var (writes_var (fst (get var))) ->
+  CSL (fun _ => default nt) tid
+    (!(var === val) ** !(pure (0 <= val /\ val < Zn len))%Z ** input_spec env env_den (perm_n nt_gr))
+    (fst (get var))
+    (!((snd (get var)) ==t (get_den val)) ** input_spec env env_den (perm_n nt_gr)).
+
+(* dimension *)
+Hypothesis get_den_length :
+  forall v, length (get_den v) = inDim.
+Hypothesis get_length :
+  forall v, length (snd (get v)) = inDim.
+
+(* code generators filling the function hole *)
+(* func : the argument variable ->
+    the command for getting the result and the return expression  *)
+Variable f_den : list val -> list val.
+
+Hypothesis func_fv :
+  forall v, disjoint [I; BID] (writes_var (fst (func v))) .
+Hypothesis func_no_bar :
+  forall v, barriers (fst (func v)) = nil.
+Hypothesis func_fv_sh :
+  forall u v, List.In u (writes_var (fst (func v))) -> prefix "sh" (var_of_str u) = false.
+Hypothesis func_fv_arr :
+  forall u v, List.In u (writes_var (fst (func v))) -> prefix "arr" (var_of_str u) = false.
+Hypothesis func_fv_x :
+  forall u v, List.In u (writes_var (fst (func v))) -> prefix "x" (var_of_str u) = false.
+
+(* {v == val} func {ret == f_den val} *)
+Hypothesis func_denote : forall (var : list var) nt (tid : Fin.t nt) (val : val),
+  length var = inDim ->
+  disjoint var (writes_var (fst (func var))) ->
+  CSL (fun _ => default nt) tid
+    ( !(pure (0 <= val /\ val < Zn len)%Z) **
+      !(vars2es var ==t (get_den val)) ** input_spec env env_den (perm_n nt_gr))
+    (fst (func var))
+    (!((snd (func var)) ==t (f_den (get_den val))) ** input_spec env env_den (perm_n nt_gr)).
+
+Hypothesis fout_length :
+  forall i, length (fout i) = outDim.
+Hypothesis fden_length :
+  forall v, length (f_den v) = outDim.
+Hypothesis out_length :
+  length out = outDim.
+Hypothesis func_length :
+  forall v, length (snd (func v)) = outDim.
+
+Section block_verification.
+Variable bid : Fin.t nblk.
+
+Notation zf i := (Z_of_fin i).
+
+Section thread_verification.
+Variable tid : Fin.t ntrd.
+
+Notation gtid := (nf tid + nf bid * ntrd).
+
+Open Scope string.
+
+Notation GOuts := (es2gls Outs).
+Notation gl_out := (es2gls (vs2es out)).
+
+Definition inv :=
+  Ex ix, 
+    !(Outs ==t out) **
+    !(Len === Zn len) **
+    !(I === Enum' (ix * nt_gr + gtid)) **
+    !(Apure (ix * nt_gr + gtid < len + nt_gr)%nat) **
+    input_spec env env_den (perm_n nt_gr) **
+    nth gtid (distribute_tup nt_gr gl_out (ix * nt_gr) (fun i => (f_den (get_den (Zn i))))%Z (nt_step nt_gr) 0 1%Qc) emp **
+    nth gtid (distribute_tup nt_gr gl_out (len - (ix * nt_gr)) (fun i => fout i) (nt_step nt_gr) (ix * nt_gr) 1%Qc) emp.
+
+Notation GTID := (TID +C BID *C Zn ntrd).
+
+Hint Rewrite Nat2Z.inj_add Nat2Z.inj_mul Nat2Z.inj_succ div_Zdiv : sep.
+
+Hint Unfold Len Outs writeArray name_of_len.
+
+Open Scope string.
+
+Arguments append _ _ : simpl never.
+
+Lemma nt_gr_neq_0 : nt_gr <> 0.
+nia.
+Qed.
+
+Hint Resolve nt_gr_neq_0.
+
+Lemma map_correct : 
+  CSL (fun n => default ntrd) tid
+   (!(Outs ==t out) **
+   !(Len === Zn len) **
+   (input_spec env env_den (perm_n nt_gr)) **
+   List.nth (nf tid + nf bid * ntrd) (distribute_tup nt_gr gl_out len fout (nt_step nt_gr) 0 1%Qc) emp **
+   !(BID === zf bid) ** !(TID === zf tid))
+
+  (map_ker inv)
+
+  ( input_spec' env_den (perm_n nt_gr) **
+    List.nth gtid (distribute_tup nt_gr gl_out len (fun v=>(f_den (get_den (Zn v))))%Z (nt_step nt_gr) 0 1%Qc) emp).
+Proof.
+  unfold map_ker.
+  eapply rule_seq.
+  { hoare_forward; intros ? ? H'.
+    destruct H' as [v H'].
+    subA_normalize_in H' with ( fun H => first
+      [ apply subA_distribute_tup in H | apply subA_eq_tup in H
+      | apply subA_is_tuple_p in H | apply subA_input_spec in H; eauto ] ).
+    repeat subE_simpl in *. simpl in H'. autounfold in H'. simpl in H'.
+    rewrite subE_vars2es in H'; auto.
+    exact H'. }
+  hoare_forward.
+  { unfold inv; eapply Hbackward.
+    Focus 2.
+    { intros s h H; apply ex_lift_l_in in H as [x H]; sep_split_in H.
+      change_in H.
+      { unfold_pures.
+        sep_rewrite_in skip_arr_tup_unfold' H; [|try first [omega | eauto]..].
+        2: nia.
+        (* sep_rewrite_in (@is_array_unfold (Gl arr) (x * nt_gr + gtid)) H; [|try first [omega | eauto]..]. *)
+        (* 2: nia. *)
+        (* rewrite <-plus_n_O in H. *)
+      apply H. } 
+      sep_combine_in H. ex_intro x H. simpl in H. exact H. } Unfocus.
+    
+    hoare_forward.
+    eapply rule_seq. 
+    { autorewrite with sep. eapply Hbackward. 
+      Focus 2.
+      { intros s h H.
+        sep_split_in H.
+        change_in H.
+        { assert (((Zn x * (Zn nblk * Zn ntrd) + (zf tid + zf bid * Zn ntrd))%Z === I)%exp
+                      s (emp_ph loc)).
+          { unfold_pures; unfold_conn; simpl; nia. }
+          sep_rewrite_in (mps_eq1_tup') H; [|exact H0]. 
+          sep_combine_in H; exact H. }
+        evar (P : assn).
+        assert (((input_spec env env_den (1 / injZ (Zn nblk * Zn ntrd)) **
+                 !(pure (0 <= (Zn x * (Zn nblk * Zn ntrd) + (zf tid + zf bid * Zn ntrd)) < Zn len))%Z **
+                 !(I === (Zn x * (Zn nblk * Zn ntrd) + (zf tid + zf bid * Zn ntrd))%Z)) ** P) s h).
+        { sep_normal; repeat sep_cancel.
+          sep_split; [sep_split_in H1; unfold_pures; unfold_conn; simpl in *; nia|].
+          unfold P; eauto. }
+        unfold P in *; apply H0. } Unfocus.
+      apply rule_frame.
+      { eapply Hbackward; [apply get_denote; lets: (>>get_fv I); simpl in *; jauto|].
+        intros.
+        sep_split_in H; sep_split; eauto.
+        unfold_pures; unfold_conn; simpl in *.
+        autorewrite with sep; auto. }
+      destructs (get_fv I).
+      repeat prove_inde;
+      try (first [apply disjoint_indeE | apply disjoint_indelE | apply disjoint_indeB]; simpl;
+           repeat split; eauto );
+      try (intros Hc; apply get_fv_sh in Hc; simpl in Hc; congruence);
+      first [apply inde_distribute_tup | apply inde_is_tup |
+             apply inde_eq_tup ]; apply Forall_forall;
+      intros; first [apply indeE_fv|apply indelE_fv]; intros Hc;
+      lazymatch goal with
+        | [H : In _ (writes_var (fst (get _))) |- _] => lets: (>>get_fv_sh H); lets: (>>get_fv_arr H)
+      end;  unfold tarr_idx, es2gls, vs2es in *.
+      
+      { eapply outs_prefix in H2; eauto; try congruence. 
+        congruence. }
+      { repeat apply in_map_iff in H2 as [? [? H2]]; subst; simpl in Hc; 
+        destruct Hc. }
+      { repeat apply in_map_iff in H2 as [? [? H2]]; subst;
+        simpl in Hc; destruct Hc as [|[]]; subst; eauto. }
+      { repeat apply in_map_iff in H2 as [? [? H2]]; subst; simpl in Hc; destruct Hc. }
+      { repeat apply in_map_iff in H2 as [? [? H2]]; subst; simpl in Hc; destruct Hc. } }
+      
+      (* hoare_forward; try (apply inde_distribute; auto; repeat (constructor; prove_indeE)); simpl. *)
+      (* apply inde_eq_tup. *)
+      (* apply outs_inde; rewrite Forall_forall; simpl; intros ? [? | ?]; subst; simpl; tauto. *)
+      (* apply inde_distribute_tup. *)
+      (* apply inde_vals_l. *)
+      (* apply inde_is_tup. *)
+      
+      (* Lemma inde_tarr_idx es ix vs : *)
+      (*   Forall (fun e : loc_exp => forall v, In v vs -> indelE e v) es -> *)
+      (*   (forall v, In v vs -> indeE ix v) -> *)
+      (*   Forall (fun e : loc_exp => forall v : var, In v vs -> indelE e v) *)
+      (*          (tarr_idx es ix). *)
+      (* Proof. *)
+      (*   unfold tarr_idx; rewrite !Forall_forall. *)
+      (*   intros Hes Hix x Hx. *)
+      (*   apply in_map_iff in Hx as [? [? Hx]]; subst. *)
+      (*   intros. *)
+      (*   forwards: (>> Hix H). *)
+      (*   forwards: (>>Hes Hx H). *)
+      (*   prove_indeE; rewrite <-H0, <-H1; auto. *)
+      (* Qed. *)
+
+      (* apply inde_tarr_idx. *)
+      (* apply inde_vals_l. *)
+      (* simpl; destruct 1; try tauto. *)
+      (* subst; prove_inde. *)
+      (* apply inde_vals. *)
+      (* apply inde_distribute_tup. *)
+      (* apply inde_vals_l. *)
+      (* intros ? ? H; apply H. } *)
+
+    eapply rule_seq.
+    { eapply Hbackward; [|intros ? ? H; sep_normal_in H; eauto].
+      apply rule_frame.
+      apply read_tup_correct.
+      intros; intros Hc.
+      eapply get_res_fv in Hc; apply locals_pref in H; eauto; congruence.
+
+      apply locals_disjoint_ls.
+      rewrite get_den_length, get_length; auto.
+      unfold xs; rewrite locals_length, get_length; auto.
+      rewrite read_tup_writes; [|unfold xs; rewrite locals_length, get_length; auto].
+      unfold xs.
+      lets Hpref: (>>locals_pref "x" inDim).
+
+      repeat prove_inde;
+      try (first [apply disjoint_indeE | apply disjoint_indelE | apply disjoint_indeB]; simpl;
+           repeat split; eauto );
+      try (intros Hc; apply Hpref in Hc; simpl in Hc; congruence);
+      first [apply inde_distribute_tup | apply inde_is_tup |
+             apply inde_eq_tup | apply inde_input_spec]; try (apply Forall_forall;
+      intros; first [apply indeE_fv|apply indelE_fv]; intros Hc;
+      lazymatch goal with
+        | [H : In _ (locals _ _) |- _] => lets: (>>Hpref H)
+      end;  unfold tarr_idx, es2gls, vs2es in *).
+      
+      { intros; lets: (>>Hpref ___); eauto; apply prefix_ex in H0 as [? ?]; rewrite H0; simpl; auto. }
+      { intros; lets: (>>Hpref ___); eauto; apply prefix_ex in H0 as [? ?]; rewrite H0; simpl; auto. }
+      { eapply outs_prefix in H; eauto.
+        apply prefix_ex in H1 as [? ?]; rewrite H1 in H; simpl in H; congruence. }
+      { repeat apply in_map_iff in H as [? [? H]]; subst; simpl in Hc; destruct Hc. }
+      { repeat apply in_map_iff in H as [? [? H]]; subst; simpl in Hc.
+        destruct Hc as [Hc|[]]; subst; simpl in H1; congruence. }
+      { repeat apply in_map_iff in H as [? [? H]]; subst; simpl in Hc; destruct Hc. }
+      { repeat apply in_map_iff in H as [? [? H]]; subst; simpl in Hc; destruct Hc. } }
+      
+    eapply rule_seq.
+    { (* executute the passed function *)
+      eapply Hbackward.
+      Focus 2. { 
+        intros s h H.
+        evar (Q : assn);
+        assert (((!(pure (0 <= Zn x * (Zn nblk * Zn ntrd) + (zf tid + zf bid * Zn ntrd) < Zn len))%Z **
+                  !(vars2es xs ==t get_den
+                    (Zn x * (Zn nblk * Zn ntrd) + (zf tid + zf bid * Zn ntrd))%Z) **
+                  input_spec env env_den (perm_n nt_gr)) **Q) s h).
+        { sep_split; sep_normal; repeat sep_cancel; unfold Q; eauto.
+          sep_split; [sep_split_in H1; unfold_pures; unfold_conn; simpl; nia|].
+          exact H1. }
+        unfold Q in *; clear Q; exact H0. } Unfocus.
+      apply rule_frame.
+      { apply func_denote.
+        unfold xs; rewrite locals_length; auto.
+        apply disjoint_comm, not_in_disjoint; intros x0 H Hc.
+        lets: (>>func_fv_x H).
+        apply locals_pref in Hc; congruence. }
+      lets: (func_fv xs); simpl in *.
+      repeat prove_inde;
+      try (first [apply disjoint_indeE | apply disjoint_indelE | apply disjoint_indeB]; simpl;
+           repeat split; jauto );
+      try (intros Hc; apply func_fv_sh in Hc; simpl in Hc; congruence);
+      first [apply inde_distribute_tup | apply inde_is_tup |
+             apply inde_eq_tup | apply inde_input_spec ]; apply Forall_forall;
+      intros; first [apply indeE_fv|apply indelE_fv]; intros Hc;
+      lazymatch goal with
+        | [H : In _ (writes_var (fst (func _))) |- _] => lets: (>>func_fv_sh H); lets: (>>func_fv_arr H)
+      end;  unfold tarr_idx, es2gls, vs2es in *.
+      { eapply outs_prefix in H0; eauto. congruence. }
+      { repeat apply in_map_iff in H0 as [? [? H0]]; subst; simpl in Hc; destruct Hc.  }
+      { repeat apply in_map_iff in H0 as [? [? H0]]; subst; simpl in Hc; destruct Hc as [|[]]; subst; jauto. }
+      { repeat apply in_map_iff in H0 as [? [? H0]]; subst; simpl in Hc; destruct Hc. }
+      { repeat apply in_map_iff in H0 as [? [? H0]]; subst; simpl in Hc; destruct Hc. } }
+
+    eapply rule_seq.
+    { (* set the results to output array *)
+      eapply Hbackward.
+      Focus 2. {
+        intros s h H.
+        sep_split_in H.
+        sep_rewrite_in_r mps_eq1_tup H; [|eauto].
+        sep_combine_in H.
+        sep_lift_in H 7; exact H.
+      } Unfocus.
+      apply rule_frame.
+      apply gen_write_correct; simpl.
+      unfold vs2es; rewrite map_length.
+      unfold Outs; rewrite fout_length, outs_length; auto.
+      unfold Outs; rewrite func_length, outs_length; auto.
+      
+      unfold catcmd, setOut; simpl; rewrite writes_var_gen_write.
+      intros ?; destruct 1. }
+    eapply Hforward.
+    { eapply Hbackward; [|intros s h H; sep_normal_in H; exact H].
+      hoare_forward.
+      intros ? ? H; destruct H as [v H].
+      sep_normal_in H.
+      subA_normalize_in H with ( fun H => first
+      [ apply subA_distribute_tup in H | apply subA_eq_tup in H
+      | apply subA_is_tuple_p in H | apply subA_input_spec in H; eauto ] ). simpl in H.
+      unfold Outs in *; simpl in H.
+      repeat (rewrite !subE_vars2es in H; eauto).
+      assert ((subEs I v (snd (func xs)) ==t
+              f_den (get_den
+               (Zn x * (Zn nblk * Zn ntrd) + (zf tid + zf bid * Zn ntrd))%Z)) s (emp_ph loc)).
+      { sep_split_in H; unfold_pures; eauto. }
+      sep_rewrite_in mps_eq2_tup H; [|exact H0].
+      subE_simpl in *.
+      rewrite sublEs_tarr_idx in H.
+      ex_intro v H. exact H. }
+    
+    unfold inv; intros s h H. destruct H as (v & H); simpl in H.
+    sep_normal_in H; sep_split_in H.
+    unfold_pures; subst.
+    unfold Outs, writeArray, names_of_arg; simpl.
+    exists (S x); autorewrite with sep.
+    sep_split; try now (unfold_conn; simpl; auto; omega).
+    { rewrite <-out_length; auto. }
+    { unfold_conn; simpl. rewrite HP5. ring. }
+    autorewrite with sep in H. sep_cancel.
+    (* sep_rewrite (@is_array_unfold (Gl arr) (x * nt_gr + gtid)); try omega; eauto. *)
+    lets Heq: (sublEs_es2gls); unfold es2gls in Heq; rewrite !Heq in H.
+    rewrite subE_vars2es in H; auto.
+    sep_rewrite_r (@skip_arr_tup_fold' (nf tid + nf bid * ntrd) gl_out); try omega; eauto.
+    sep_normal; simpl.
+    simpl; repeat sep_cancel.
+    cuts_rewrite (len - (nt_gr + x * nt_gr) = len - x * nt_gr - nt_gr); [|nia].
+    sep_rewrite_r mps_eq1_tup; [|apply HP1].
+    lets Hrw: sublEs_es2gls; unfold es2gls in Hrw; rewrite Hrw in H1.
+    rewrite subEs_ss2es in H1; eauto.
+    repeat autorewrite with sep. repeat sep_cancel.
+    intros ? Hout; apply names_of_array_in in Hout; intros Hc; subst; simpl in Hout; congruence. }
+  { unfold inv; intros s h H. apply ex_lift_l_in in H as [x H]. sep_split_in H. unfold_pures.
+    rewrite HP1, HP2 in n; rewrite <-Nat2Z.inj_lt in n.
+    assert (len - x * nt_gr <= nf tid + nf bid * ntrd) by (zify; omega).
+    assert (nf tid + nf bid * ntrd < nt_gr) by auto.
+    sep_cancel.
+    revert H; apply scRw_stack; intros h' H.
+    apply input_spec_forget in H; eauto.
+    (* apply scC in H; sep_rewrite_in nth_dist_nil H; try omega; eauto. *)
+    (* 2: instantiate (1 :=len - x * nt_gr); intros j Hj; unfold nt_step. *)
+    (* 2: rewrite plus_comm, Nat.mod_add; auto; rewrite Nat.mod_small; auto; try (zify; omega). *)
+    sep_lift_in H 1; sep_rewrite_in nth_dist_nil_tup H; try omega; eauto.
+    
+    2: instantiate (1 :=len - x * nt_gr); intros j Hj; unfold nt_step.
+    2: rewrite plus_comm, Nat.mod_add; auto; rewrite Nat.mod_small; auto; try (zify; omega).
+    rewrite minus_diag in H; simpl in H.
+    rewrite nth_nseq in H.
+    assert (x * nt_gr <= len \/ len < x * nt_gr) as [|] by omega.
+    - apply scC in H; sep_rewrite_in nth_dist_tup_ext H; try omega; auto.
+      2: instantiate (1 :=len - x * nt_gr); intros j Hj; simpl; unfold nt_step;
+         rewrite plus_comm, Nat.mod_add; auto; rewrite Nat.mod_small; auto; try omega.
+      sep_normal_in H.
+      (* sep_rewrite_in nth_dist_ext H2; try omega; auto. *)
+      (* 2: instantiate (1 :=len - x * nt_gr); intros j Hj; simpl; unfold nt_step. *)
+      (* 2: rewrite plus_comm, Nat.mod_add; auto; rewrite Nat.mod_small; auto; try omega. *)
+      cutrewrite (x * nt_gr + (len - x * nt_gr) = len) in H; [|omega].
+      destruct Compare_dec.leb; sep_normal_in H; sep_split; try now (unfold_conn; simpl; auto); sep_cancel.
+    - (* apply scC in H2; sep_rewrite nth_dist_ext; try omega; auto. *)
+      (* cutrewrite (len - x * ntrd = 0) in H2; [|omega]. *)
+      cutrewrite (x * nt_gr = len + (x * nt_gr - len)) in H; [|omega].
+      assert (forall j, j < x * nt_gr - len -> nt_step nt_gr (0 + len + j) <> nf tid + nf bid * ntrd).
+      { unfold nt_step; simpl; intros j Hj Hc.
+        assert (len + j + nt_gr < (S x) * nt_gr) by (simpl; omega).
+        assert (x * nt_gr + j + (nf tid + nf bid * ntrd) < len + j + nt_gr) by omega.
+        let t := (eval simpl in (Nat.mod_add (len + j) 1 nt_gr)) in pose proof t.
+        rewrite mult_1_l in H5.
+        rewrite (Nat.div_mod (len + j + nt_gr) nt_gr), H5 in H3, H4; auto.
+        assert (x * nt_gr  < nt_gr * ((len + j + nt_gr) / nt_gr)) by omega.
+        assert (nt_gr * ((len + j + nt_gr) / nt_gr) < S x * nt_gr) by omega.
+        rewrite mult_comm in H6; apply Nat.mul_lt_mono_pos_l in H6; try omega.
+        rewrite mult_comm in H7; apply Nat.mul_lt_mono_pos_r in H7; omega. } 
+      sep_rewrite_in_r nth_dist_tup_ext H; try omega; eauto.
+      sep_split; auto.
+      destruct Compare_dec.leb; sep_normal_in H; repeat sep_cancel. }
+
+  {  intros s h H; unfold inv; exists 0; simpl.
+     sep_split_in H; unfold_pures; sep_split; auto.
+     - unfold_conn; simpl; autorewrite with sep. unfold_conn_in HP; simpl in HP. 
+       repeat match goal with [H : _ = _|- _] => first [rewrite <-H | rewrite H]; clear H end; auto.
+     - unfold_conn. assert (nf tid + nf bid * ntrd < nt_gr) by auto. omega.
+     - rewrite <-minus_n_O, nth_nseq; destruct Compare_dec.leb; sep_normal; sep_cancel. }
+Qed.
+End thread_verification.
+
+Require Import Bdiv.
+Local Notation init := MyVector.init.
+Definition bth_pre :=
+  !(Outs ==t out) **
+  !(Len === Zn len) **
+  conj_xs (ls_init 0 ntrd (fun i => input_spec env env_den (perm_n nt_gr))) **
+  conj_xs (ls_init 0 ntrd (fun i =>
+    nth (i + nf bid * ntrd)
+    (distribute_tup nt_gr (es2gls (vs2es out)) len fout (nt_step nt_gr) 0 1) emp)).
+
+Definition tr_pres := init (fun i : Fin.t ntrd =>
+  !(Outs ==t out) ** 
+  !(Len === Zn len) **
+  input_spec env env_den (perm_n nt_gr) **
+  nth (nf i + nf bid * ntrd)
+    (distribute_tup nt_gr (es2gls (vs2es out)) len fout (nt_step nt_gr) 0 1) emp **
+  !(BID === zf bid)).
+
+Definition bth_post  :=
+  conj_xs (ls_init 0 ntrd (fun i => input_spec' env_den (perm_n nt_gr))) **
+  conj_xs (ls_init 0 ntrd (fun i =>
+    nth (i + nf bid * ntrd)
+      (distribute_tup nt_gr (es2gls (vs2es out)) len
+        (fun v : nat => f_den (get_den (Zn v))) (nt_step nt_gr) 0 1) emp)).
+
+Definition tr_posts := (init (fun i : Fin.t ntrd =>
+  input_spec' env_den (perm_n nt_gr) **
+  nth (nf i + nf bid * ntrd)
+    (distribute_tup nt_gr (es2gls (vs2es out)) len
+      (fun v : nat => f_den (get_den (Zn v))) (nt_step nt_gr) 0 1) emp)).
+
+Definition out_vars := List.map Var (names_of_array "Out" outDim).
+
+Definition E : Lang.env := fun v =>
+  if var_eq_dec v BID then Lo
+  else if prefix "sh" (var_of_str v) then Lo
+  else if prefix "arr" (var_of_str v) then Lo
+  else Hi.  
+Close Scope Qc_scope.
+Close Scope Q_scope.
+(* delete arguments of map_ker *)
+Definition tid0 : Fin.t ntrd.
+destruct ntrd; try omega.
+exact Fin.F1.
+Qed.
+
+Definition map' : cmd.
+  pose (map_ker FalseP) as map'; unfold map_ker, WhileI in map'; exact map'.
+Defined.
+
+Definition bspec : (barrier_spec ntrd) := fun i => (default ntrd).
+
+Lemma precise_false : precise (fun _ _ => False).
+Proof.
+  unfold precise; intros; tauto.
+Qed.
+
+Lemma map_correct_b :
+  CSLp ntrd E (bth_pre ** !(BID === zf bid)) map' (bth_post).
+Proof.
+  applys (>> rule_par bspec tr_pres tr_posts).
+  - destruct ntrd; eexists; try omega; eauto.
+  - unfold bspec; split; intros; unfold default; simpl; rewrite MyVector.init_spec;
+    unfold CSL.low_assn, low_assn, indeP; tauto.
+  - eauto.
+  - split; unfold bspec, default; simpl; rewrite MyVector.init_spec;
+    apply precise_false.
+  - unfold bth_pre, tr_pres; intros.
+    sep_split_in H.
+    istar_simplify.
+    repeat sep_rewrite (@ls_star).
+    repeat sep_rewrite (@ls_pure).
+    sep_split.
+    apply ls_emp'; intros; rewrite ls_init_spec; destruct lt_dec; auto; cbv; auto.
+    apply ls_emp'; intros; rewrite ls_init_spec; destruct lt_dec; auto; cbv; auto.
+    apply ls_emp'; intros; rewrite ls_init_spec; destruct lt_dec; auto; cbv; auto.
+    repeat sep_cancel.
+  - unfold tr_posts, bth_post; intros s h H.
+    istar_simplify_in H.
+    sep_cancel.
+    
+  - intros; unfold tr_pres; rewrite MyVector.init_spec.
+    unfold CSL.low_assn.
+    repeat prove_low_assn; eauto.
+    apply low_assn_eqt.
+    apply Forall_forall; intros.
+    
+    unfold Outs, writeArray, names_of_arg, ss2es, names_of_array in H; simpl in H.
+    rewrite in_map_iff in H; destruct H as [? [? ?]]; subst.
+
+    rewrite In_ls_init in H0; destruct H0 as [z [? ?]]; subst.
+    constructor; unfold E; simpl; auto.
+    constructor; eauto.
+
+    apply low_assn_input_spec.
+    intros; unfold E; rewrite H; repeat destruct var_eq_dec; eauto.
+    destruct (prefix "sh"); auto.
+    intros; unfold E; rewrite H; repeat destruct var_eq_dec; eauto.
+    apply low_assn_skip_arr_tup.
+    rewrite Forall_forall; unfold es2gls, vs2es; intros.
+    repeat (rewrite in_map_iff in H; destruct H as [? [? H]]; subst).
+    repeat constructor.
+  - intros; unfold CSL.low_assn, tr_posts; rewrite MyVector.init_spec.
+    repeat prove_low_assn.
+
+    apply low_assn_input_spec'.
+    (* intros; unfold E; rewrite H; repeat destruct var_eq_dec; eauto. *)
+    (* destruct (prefix "sh"); auto. *)
+    (* intros; unfold E; rewrite H; repeat destruct var_eq_dec; eauto. *)
+    apply low_assn_skip_arr_tup.
+    apply Forall_forall; intros ? H. unfold es2gls, vs2es in H.
+    repeat (rewrite in_map_iff in H; destruct H as [? [? H]]; subst).
+    repeat constructor.
+  - repeat (match goal with
+            | [ |- typing_exp _ _ _ ] => eapply ty_var; apply le_type_refl
+            | _ => econstructor
+            end); try reflexivity.
+    repeat instantiate (1 := Hi).
+    apply typing_cmd_Hi; eauto.
+    intros.
+    unfold E; repeat destruct var_eq_dec; subst; lets: (get_fv I); simpl in *; try tauto.
+    destruct (prefix "sh" (var_of_str v)) eqn:Heq.
+    apply get_fv_sh in H; congruence.
+    destruct (prefix "arr" (var_of_str v)) eqn:Heq'; auto.
+    apply get_fv_arr in H; congruence.
+    
+    apply read_tup_hi.
+    unfold xs; intros.
+    apply locals_pref in H; unfold E.
+    repeat (destruct (var_eq_dec); subst; simpl in H; try congruence).
+    apply prefix_ex in H as [? ?]; rewrite H.
+    simpl; eauto.
+
+    apply typing_cmd_Hi; eauto.
+    intros; unfold E.
+    lets: (>>disjoint_not_in_r v (func_fv xs) H).
+    lets: (>>func_fv_arr v xs H).
+    lets: (>>func_fv_sh v xs H).
+    destruct var_eq_dec; subst.
+    elimtype False; apply H0; simpl; eauto.
+    rewrite H1, H2; eauto.
+    
+    apply typing_cmd_Hi.
+    apply gen_write_no_bars.
+    unfold catcmd, setOut, writeArray; simpl; intros ?; rewrite writes_var_gen_write; simpl; try tauto.
+  - unfold tr_pres, tr_posts; intros; rewrite !MyVector.init_spec.
+    unfold bspec, skip_arr.
+    eapply Hbackward.
+    eapply Hforward.
+    apply map_correct.
+    intros.
+
+    apply H.
+    intros; sep_normal_in H; sep_normal; repeat sep_cancel.
+    (* hmm.. *)
+    Grab Existential Variables.
+    apply Lo.
+    apply Lo.
+    apply Lo.
+    apply 0.
+Qed.
+
+End block_verification.
+
+Definition bl_pres : Vector.t assn nblk :=
+  MyVector.init (fun b : Fin.t nblk => (bth_pre b)).
+Definition bl_posts : Vector.t assn nblk :=
+  MyVector.init (fun b : Fin.t nblk => (bth_post b)).
+
+Definition bid0 : Fin.t nblk.
+  destruct nblk; try omega.
+  exact Fin.F1.
+Qed.
+
+Theorem map_correct_g  :
+  CSLg ntrd nblk ntrd_neq0 nblk_neq0
+    (!(Outs ==t out) ** !(Len === Zn len) **
+     input_spec env env_den 1 ** is_tuple_array_p (es2gls (vs2es out)) len fout 0 1)
+
+    (Pr nil map')
+
+    (input_spec' env_den 1 ** is_tuple_array_p (es2gls (vs2es out)) len (fun v => f_den (get_den (Zn v)))%Z 0 1).
+Proof.
+  applys (>> rule_grid E bl_pres bl_posts).
+  - intros s h H.
+    unfold bl_pres, bth_pre.
+    sep_split_in H.
+    istar_simplify.
+    repeat sep_rewrite (@ls_star nblk).
+    repeat sep_rewrite (@ls_pure nblk); sep_split.
+    apply ls_emp'; intros; rewrite ls_init_spec; destruct lt_dec; auto; cbv; auto.
+    apply ls_emp'; intros; rewrite ls_init_spec; destruct lt_dec; auto; cbv; auto.
+    (* apply ls_emp'; intros; rewrite ls_init_spec; destruct lt_dec; auto; cbv; auto. *)
+    repeat (sep_rewrite_r is_array_skip_arr); sep_cancel; eauto.
+    
+    sep_rewrite conj_xs_init_flatten; simpl.
+    
+    sep_rewrite input_spec_p1; eauto; try nia.
+    intros; simpl; unfold es2gls, vs2es; rewrite !map_length, fout_length.
+    unfold val in *; rewrite out_length; auto.
+  - unfold bl_pres, bl_posts; intros.
+    rewrite !MyVector.init_spec.
+    eapply CSLp_backward.
+    eapply CSLp_forward.
+    apply (map_correct_b bid).
+    intros; simpl; sep_normal; eauto.
+    intros; simpl in *; sep_normal_in H; eauto.
+  - unfold bl_posts, bth_post in *.
+    intros s h H.
+    istar_simplify_in H.
+    sep_rewrite_in conj_xs_init_flatten H; simpl in H.
+    (* lets Heq: (>>is_array_is_array_p_1 __ __ nt_gr); sep_rewrite Heq; eauto; try nia. *)
+    sep_rewrite_in input_spec'_p1 H; eauto; try nia.
+    sep_rewrite is_array_skip_arr; eauto.
+    unfold es2gls, vs2es, val in *; rewrite !map_length; intros.
+    rewrite out_length, fden_length; auto.
+  - prove_inde.
+  - intros; unfold bl_pres, bth_pre.
+    rewrite MyVector.init_spec.
+    prove_inde.
+    apply inde_eq_tup, Forall_forall.
+    intros.
+    apply indeE_fv; intros Hc.
+    eapply outs_prefix in H; eauto.
+    simpl in H0; repeat destruct H0 as [|H0]; subst; simpl in H; congruence.
+    (* apply inde_eq_tup, Forall_forall; unfold Outs, writeArray, names_of_arg; simpl; intros x H. *)
+    (* unfold vars2es, names_of_array in H; *)
+    (*   rewrite in_map_iff in H; destruct H as [? [? H]]; subst; rewrite In_ls_init in H; *)
+    (*   destruct H as [? [? ?]]; subst. *)
+    (* intros; destruct H as [? | [? | ?]]; try tauto; subst; *)
+    (* prove_indeE. *)
+    apply inde_conj_xs; rewrite init_length; intros;
+    rewrite ls_init_spec; destruct lt_dec; prove_inde.
+    apply inde_input_spec; intros v; destruct 1 as [|[|[]]]; subst; simpl; auto.
+    apply inde_conj_xs; rewrite init_length; intros;
+    rewrite ls_init_spec; destruct lt_dec; prove_inde; simpl.
+    apply inde_distribute_tup; rewrite Forall_forall.
+    intros; apply indelE_fv; intros Hc.
+    unfold es2gls, vs2es in H0; repeat (apply in_map_iff in H0 as [? [? H0]]; subst).
+    simpl in Hc; auto.
+  - intros bid; unfold bl_pres, bth_pre; rewrite MyVector.init_spec.
+    Hint Constructors typing_exp typing_lexp.
+    repeat prove_low_assn; eauto.
+    apply low_assn_eqt. unfold Outs.
+    rewrite Forall_forall.
+    intros x H; apply writeArray_vars in H.
+    destruct H as [? [? H]]; subst.
+    constructor; unfold E.
+    unfold var_of_str. rewrite H.
+    repeat lazymatch goal with [|- context [if ?X then _ else _]] => destruct X; auto end.
+    jauto.
+    constructor; eauto.
+    apply low_assn_conj_xs; rewrite init_length; intros.
+    rewrite ls_init_spec; destruct lt_dec; try repeat prove_low_assn.
+    apply low_assn_input_spec.
+    unfold E; intros ? ->; repeat (lazymatch goal with [|- context [if ?B then _ else  _]] => destruct B; eauto end).
+    unfold E; intros ? ->; repeat (lazymatch goal with [|- context [if ?B then _ else  _]] => destruct B; eauto end).
+    apply low_assn_conj_xs; rewrite init_length; intros.
+    rewrite ls_init_spec; destruct lt_dec; try repeat prove_low_assn.
+    apply low_assn_skip_arr_tup.
+    rewrite Forall_forall; intros ? He.
+    unfold es2gls, vs2es in He.
+    repeat (rewrite in_map_iff in He; destruct He as [? [? He]]; subst).
+    eauto.
+  - intros.
+    unfold bl_posts, bth_post.
+    rewrite MyVector.init_spec.
+    has_no_vars_assn; apply has_no_vars_conj_xs; rewrite init_length; intros; rewrite ls_init_spec;
+    repeat has_no_vars_assn.
+    
+    apply has_no_vars_input_spec.
+    apply has_no_vars_skip_arr_tup; repeat constructor.
+    unfold es2gls, vs2es.
+    rewrite Forall_forall; rewrite map_map; intros ? H'; rewrite in_map_iff in H';
+    destruct H' as [? [? ?]]; subst; prove_inde.
+  - simpl; tauto.
+  - unfold E; eauto.
+  - unfold E; eauto.
+  - eauto.
+  - eauto.
+  - simpl; eauto.
+Qed.
+    
+End Map.
+
