pmap_skel_test.v
@@ -1,0 +1,215 @@
+Require Import GPUCSL.
+Require Import pmap_ske.
+Require Import Skel_lemma.
+Require Import scan_lib.
+Require Import LibTactics.
+Require Import Psatz.
+
+Section verification_example.
+  Variable ntrd : nat.
+  Variable nblk : nat.
+  
+  Hypothesis ntrd_neq_0 : ntrd <> 0.
+  Hypothesis nblk_neq_0 : nblk <> 0.
+
+  Open Scope list.
+  Open Scope string.
+  Close Scope exp.
+  Eval compute in names_of_arg (grpOfInt 0) 1.
+  (* length of the array: shInO, the top address of the array: arrInOO *)
+  Definition env := (0, 1) :: (1, 1) :: nil.
+  Eval compute in names_of_arg (grpOfInt 0) 1.
+  Eval compute in names_of_arg (grpOfInt 1) 1.
+  Notation t0 := (Var "lv10").
+  Notation t1 := (Var "lv11").
+
+  Notation arr0 := (Var "arrInOO").
+  Notation arr1 := (Var "arrInSOO").
+
+  Variable len : nat.
+  Hypothesis len_neq_0 : len <> 0.
+  Variable arr0_ptr : Z.
+  Variable arr1_ptr : Z.
+  Variable arr0_elms : nat -> Z.
+  Variable arr1_elms : nat -> Z.
+  Variable out_ptr : Z.
+  Variable out_elms : nat -> Z.
+  Import ListNotations.
+  Open Scope list_scope.
+  Definition arr0_elms' i := arr0_elms i :: nil.
+  Definition arr1_elms' i := arr1_elms i :: nil.
+  Definition out_elms' i := out_elms i :: nil.
+  
+  Definition env_den := (arr0_ptr :: nil, len, arr0_elms') ::
+                        (arr1_ptr :: nil, len, arr1_elms') :: nil.
+  Definition out_ptr' := out_ptr :: nil.
+  
+  Definition default_var := Var "".
+
+  Definition inDim := 2.
+  Definition get (x : var) :=
+    ( t0 ::= x ;; t1 ::= [Gl arr0 +o x], Evar t0 :: Evar t1 :: nil).
+
+  Definition get_den val := val :: (arr0_elms (Z.to_nat val)) :: nil.
+
+  Definition func (xs : list var) :=
+    let in0 := nth 0 xs default_var in
+    let in1 := nth 1 xs default_var in
+    ( t1 ::= [Gl arr1 +o in0 ], (in1 +C t1) :: nil).
+
+  Definition default_val := 0%Z.
+
+  Definition func_den (vals : list val) :=
+    let v0 := nth 0 vals default_val in
+    let v1 := nth 1 vals default_val in
+    (v1 + arr1_elms (Z.to_nat v0))%Z :: nil.
+
+  Definition outDim := 1.
+
+  Lemma pure_emp stk : stk ||= !(emp) <=> emp.
+  Proof.
+    split.
+    - intros; destruct H; eauto.
+    - intros; split; eauto.
+  Qed.
+
+  Theorem gen_code_correct :
+    CSLg ntrd nblk ntrd_neq_0 nblk_neq_0 
+    (!(Outs outDim ==t out_ptr :: nil) **
+     !(Len outDim === Zn len) **
+     input_spec env env_den 1 **
+     is_tuple_array_p (es2gls (vs2es out_ptr')) len out_elms' 0 1)
+    {| get_sh_decl := nil;
+       get_cmd := map' ntrd nblk inDim outDim get func |}
+    (input_spec' env_den 1 **
+     is_tuple_array_p (es2gls (vs2es out_ptr')) len (fun v : nat => func_den (get_den (Zn v))) 0 1).
+  Proof.
+    apply map_correct_g; eauto.
+    - cbv; intros.
+      repeat split; eauto; intros [? | [? | []]]; congruence.
+    - simpl.
+      intros ? ? [? | [? | []]]; subst; auto.
+    - simpl.
+      intros ? ? [? | [? | []]]; subst; auto.
+    - simpl.
+      intros ? ? ? [? | [? | []]]; subst; simpl; intros [?|[]]; subst; simpl; eauto.
+    - intros x nt tid ix Hneq. simpl in *.
+      assert (Ht0x : t0 <> x) by eauto.
+      assert (Ht1x : t1 <> x) by eauto.
+      eapply rule_seq.
+      { apply rule_frame.
+        hoare_forward.
+        - intros s h [v H].
+          remember t0.
+          subA_normalize_in H with (fun H =>  H).
+          assert ((!(t0 === ix) ** !(x === ix)) s h).
+          { sep_rewrite_in_r emp_unit_l H; sep_split_in H; sep_split.
+            unfold_conn_all; simpl in *.
+            destruct var_eq_dec; try congruence.
+            split; eauto.
+            unfold_conn_all; simpl in *.
+            destruct var_eq_dec; simpl in *; try congruence. }
+          exact H0.
+        - repeat prove_inde. }
+      eapply Hbackward.
+      Focus 2. { 
+        intros s h H.
+        sep_split_in H.
+        sep_normal_in HP1.
+        change_in H.
+        { unfold_pures.
+          sep_rewrite_in (@is_array_unfold (Gl arr0_ptr) (Z.to_nat ix)) H.
+          rewrite <-plus_n_O in H.
+          2: zify; rewrite Z2Nat.id; nia.
+          rewrite Z2Nat.id in H; [|nia].
+          assert ((Gl arr0_ptr +o ix ===l Gl arr0 +o ix) s h).
+          { unfold_conn_all; simpl in *; f_equal; omega. }
+          sep_rewrite_in mps_eq1 H; [|exact H0].
+          sep_normal_in H; exact H. }
+        sep_combine_in H.
+        exact H. } Unfocus.
+      eapply Hforward.
+      { hoare_forward; try (destruct var_eq_dec; congruence).
+        eauto. }
+      intros s h H.
+      repeat (try sep_rewrite_r sep_assoc; try sep_rewrite pure_star; try sep_rewrite pure_pure).
+      sep_rewrite pure_emp; sep_normal.
+      repeat (try sep_rewrite_in_r sep_assoc H; try sep_rewrite_in pure_star H;
+              try sep_rewrite_in pure_pure H).
+      sep_rewrite_in pure_emp H; sep_normal_in H.
+      unfold arr0_elms', fst_of_vals in *; simpl in H.
+      sep_normal_in H.
+      sep_split; sep_split_in H; eauto.
+      unfold_pures.
+      sep_rewrite (@is_array_unfold (Gl arr0_ptr) (Z.to_nat ix)); simpl.
+      2: zify; rewrite Z2Nat.id; nia.
+      sep_normal; sep_cancel.
+      rewrite <-plus_n_O, Z2Nat.id; [|nia].
+      assert ((Gl arr0_ptr +o ix ===l Gl arr0 +o ix) s h).
+      { unfold_conn_all; simpl in *; f_equal; omega. }
+      sep_rewrite mps_eq1; [|exact H1].
+      repeat sep_cancel.
+    - intros; simpl; repeat split; intros [? | ?]; eauto; congruence.
+    - simpl; intros u v [? | []]; subst; simpl; eauto.
+    - simpl; intros u v [? | []]; subst; simpl; eauto.
+    - simpl; intros u v [? | []]; subst; simpl; eauto.
+    - simpl; introv Hlen Hdis.
+      apply disjoint_comm in Hdis; simpl in Hdis; destruct Hdis as [Hdis _].
+      unfold inDim in *.
+      destruct var as [|v0 [|v1 [|? ?]]]; simpl in Hlen; try congruence.
+      simpl in Hdis.
+      assert (Hv0t1 : v0 <> t1) by eauto.
+      assert (Hv1t1 : v1 <> t1) by eauto.
+      simpl.
+      eapply Hbackward.
+      Focus 2. {
+        intros s h H.
+        repeat (try sep_rewrite_in_r sep_assoc H; try sep_rewrite_in pure_star H;
+                try sep_rewrite_in pure_pure H);
+        repeat sep_rewrite_in pure_emp H; sep_normal_in H.
+        exact H. } Unfocus.
+      eapply Hforward.
+      Focus 2. {
+        intros s h H.
+        repeat (try sep_rewrite_r sep_assoc; try sep_rewrite pure_star; try sep_rewrite pure_pure);
+          sep_rewrite pure_emp; sep_normal.
+        exact H. } Unfocus.
+      eapply Hbackward.
+      Focus 2. { 
+        intros s h H.
+        sep_split_in H.
+        change_in H. {
+          unfold_pures.
+          sep_rewrite_in (@is_array_unfold (Gl arr1_ptr) (Z.to_nat val)) H; simpl. 
+          2: zify; rewrite Z2Nat.id; nia.
+          rewrite <-plus_n_O, Z2Nat.id in H; [|nia].
+          assert ((Gl arr1_ptr +o val ===l Gl arr1 +o val) s (emp_ph loc)).
+          { unfold_conn; simpl; f_equal; congruence. }
+          sep_rewrite_in mps_eq1 H; [|exact H0].
+          sep_normal_in H; exact H. }
+        sep_combine_in H; exact H. } Unfocus.
+      eapply Hforward.
+      { hoare_forward; simpl in Hdis; [destruct var_eq_dec; try congruence..|].
+        intros s h H; sep_normal_in H; eauto. }
+      intros s h H; sep_split_in H; sep_split; eauto.
+      + unfold_pures; unfold_conn; simpl; eauto.
+        unfold fst_of_vals, arr1_elms' in *; simpl in *; congruence.
+      + sep_cancel.
+        unfold_pures.
+        sep_rewrite (@is_array_unfold (Gl arr1_ptr) (Z.to_nat val)); simpl. 
+        2: zify; rewrite Z2Nat.id; nia.
+        rewrite <-plus_n_O, Z2Nat.id; [|nia].
+        assert ((Gl arr1_ptr +o val ===l Gl arr1 +o val) s (emp_ph loc)).
+        { unfold_conn; simpl; f_equal; congruence. }
+        sep_rewrite mps_eq1; [|exact H1].
+        sep_normal; repeat sep_cancel.
+  Qed.
+
+   Goal False.
+   Proof.
+     let t := type of gen_code_correct in pose t.
+     simpl in P.
+     unfold map', map_ker, WhileI, get, func in P; simpl in P.
+   Abort.
+End verification_example.
+
